stuff

ByteBlockCacheSystem/ByteSystem.i.dfy
@@ -1,5 +1,7 @@
 include "AsyncDiskModel.s.dfy"
 include "ByteCache.i.dfy"
+include "InterpretationDisk.i.dfy"
+include "../BlockCacheSystem/BetreeJournalSystem.i.dfy"
 
 module ByteSystem refines AsyncDiskModel {
   import M = ByteCache
@@ -7,13 +9,19 @@ module ByteSystem refines AsyncDiskModel {
   import opened AsyncSectorDiskModelTypes
   import opened Maps
   import BC = BlockCache
+  import JC = JournalCache
   import BJC = BlockJournalCache
   import BJD = BlockJournalDisk
   import opened DiskLayout
   import opened JournalIntervals
+  import opened InterpretationDisk
   import opened InterpretationDiskOps
   import opened SectorType
   import opened Options
+  import opened JournalRanges
+  import BetreeJournalSystem
+  import BetreeSystem
+  import JournalSystem
 
   ///// reqWrites are correct
 
@@ -76,6 +84,7 @@ module ByteSystem refines AsyncDiskModel {
     && reqWritesHaveValidJournals(reqWrites)
     && reqWritesHaveValidSuperblocks(reqWrites)
   }
+
 
   ///// get operation from Loc
 
@@ -342,7 +351,410 @@ module ByteSystem refines AsyncDiskModel {
 
   ///////// Interpretation of the disk
 
-  function DiskNodes(disk: D.Variables) : imap<Location, Node>
+  predicate locInBounds(loc: Location, contents: seq<byte>)
   {
+    && loc.addr as int + loc.len as int <= |contents|
+  }
+
+  function atLoc(loc: Location, contents: seq<byte>) : seq<byte>
+  requires locInBounds(loc, contents)
+  {
+    contents[loc.addr .. loc.addr as int + loc.len as int]
+  }
+
+  function DiskNodesOfContents(contents: seq<byte>) : imap<Location, BC.Node>
+  {
+    imap loc |
+      && ValidNodeLocation(loc)
+      && locInBounds(loc, contents)
+      && ValidNodeBytes(atLoc(loc, contents))
+      :: NodeOfBytes(atLoc(loc, contents))
+  }
+
+  function DiskNodes(disk: D.Variables) : imap<Location, BC.Node>
+  {
+    DiskNodesOfContents(withWrites(disk.contents, disk.reqWrites))
+  }
+
+  function DiskIndirectionTablesOfContents(contents: seq<byte>) : imap<Location, IndirectionTable>
+  {
+    imap loc |
+      && ValidIndirectionTableLocation(loc)
+      && locInBounds(loc, contents)
+      && ValidIndirectionTableBytes(atLoc(loc, contents))
+      :: IndirectionTableOfBytes(atLoc(loc, contents))
+  }
+
+  function DiskIndirectionTables(disk: D.Variables) : imap<Location, IndirectionTable>
+  {
+    DiskIndirectionTablesOfContents(withWrites(disk.contents, disk.reqWrites))
+  }
+
+  predicate ValidJournalBlockBytes(bytes: seq<byte>)
+  {
+    && D.ChecksumChecksOut(bytes)
+    && JournalBytes.JournalBlockOfByteSeq(bytes).Some?
+  }
+
+  function JournalBlockOfBytes(bytes: seq<byte>) : JournalBlock
+  requires ValidJournalBlockBytes(bytes)
+  {
+    JournalBytes.JournalBlockOfByteSeq(bytes).value
+  }
+
+  function JournalBlockAt(contents: seq<byte>, i: int) : Option<JournalBlock>
+  requires 0 <= i < NumJournalBlocks() as int
+  {
+    var loc := JournalRangeLocation(i as uint64, 1);
+    if locInBounds(loc, contents)
+      && ValidJournalBlockBytes(atLoc(loc, contents))
+    then
+      Some(JournalBlockOfBytes(atLoc(loc, contents)))
+    else
+      None
+  }
+
+  function {:opaque} DiskJournalOfContentsI(contents: seq<byte>, i: int) : (res : seq<Option<JournalBlock>>)
+  requires 0 <= i <= NumJournalBlocks() as int
+  ensures |res| == i
+  ensures forall j | 0 <= j < i :: res[j] == JournalBlockAt(contents, j)
+  {
+    if i == 0 then [] else
+      DiskJournalOfContentsI(contents, i-1) + [JournalBlockAt(contents, i-1)]
+  }
+
+  function DiskJournalOfContents(contents: seq<byte>) : seq<Option<JournalBlock>>
+  {
+    DiskJournalOfContentsI(contents, NumJournalBlocks() as int)
+  }
+
+  function DiskJournal(disk: D.Variables) : seq<Option<JournalBlock>>
+  {
+    DiskJournalOfContents(withWrites(disk.contents, disk.reqWrites))
+  }
+
+  function DiskSuperblockAtLoc(contents: seq<byte>, loc: Location) : Option<Superblock>
+  requires ValidSuperblockLocation(loc)
+  {
+    if locInBounds(loc, contents)
+      && ValidSuperblockBytes(atLoc(loc, contents))
+    then Some(SuperblockOfBytes(atLoc(loc, contents)))
+    else None
+  }
+
+  function DiskSuperblock1(disk: D.Variables) : Option<Superblock>
+  {
+    DiskSuperblockAtLoc(disk.contents, Superblock1Location())
+  }
+
+  function DiskSuperblock2(disk: D.Variables) : Option<Superblock>
+  {
+    DiskSuperblockAtLoc(disk.contents, Superblock2Location())
+  }
+
+  //// Putting stuff together
+
+  function IBlockDisk(disk: D.Variables) : BlockDisk.Variables
+  {
+    BlockDisk.Variables(
+      ReqReadIndirectionTables(disk),
+      ReqReadNodes(disk),
+      ReqWriteIndirectionTables(disk),
+      ReqWriteNodes(disk),
+      DiskIndirectionTables(disk),
+      DiskNodes(disk)
+    )
+  }
+
+  function IJournalDisk(disk: D.Variables) : JournalDisk.Variables
+  requires reqWritesHaveValidSuperblocks(disk.reqWrites)
+  {
+    JournalDisk.Variables(
+      ReqReadSuperblock1(disk),
+      ReqReadSuperblock2(disk),
+      ReqReadJournals(disk),
+      ReqWriteSuperblock1(disk),
+      ReqWriteSuperblock2(disk),
+      ReqWriteJournals(disk),
+      DiskSuperblock1(disk),
+      DiskSuperblock2(disk),
+      DiskJournal(disk)
+    )
+  }
+
+  function Ik(k: Constants) : BetreeJournalSystem.Constants
+  {
+    BetreeJournalSystem.Constants(
+      AsyncSectorDiskModelConstants(BC.Constants(), BlockDisk.Constants()),
+      AsyncSectorDiskModelConstants(JC.Constants(), JournalDisk.Constants())
+    )
+  }
+
+  function I(k: Constants, s: Variables) : BetreeJournalSystem.Variables
+  requires reqWritesHaveValidSuperblocks(s.disk.reqWrites)
+  {
+    BetreeJournalSystem.Variables(
+      AsyncSectorDiskModelVariables(s.machine.bc, IBlockDisk(s.disk)),
+      AsyncSectorDiskModelVariables(s.machine.jc, IJournalDisk(s.disk))
+    )
+  }
+
+  predicate Init(k: Constants, s: Variables)
+  {
+    && D.Init(k.disk, s.disk)
+    && BetreeJournalSystem.Init(Ik(k), I(k, s))
+  }
+
+  //// Invariant stuff
+
+  predicate reqWritesHaveValidLocations(reqWrites: map<D.ReqId, D.ReqWrite>)
+  {
+    forall id | id in reqWrites ::
+        && |reqWrites[id].bytes| < 0x1_0000_0000_0000_0000
+        && ValidLocation(LocOfReqWrite(reqWrites[id]))
+  }
+
+  predicate reqReadsHaveValidLocations(reqReads: map<D.ReqId, D.ReqRead>)
+  {
+    forall id | id in reqReads ::
+        ValidLocation(LocOfReqRead(reqReads[id]))
+  }
+
+  predicate respWritesHaveValidLocations(respWrites: map<D.ReqId, D.RespWrite>)
+  {
+    forall id | id in respWrites ::
+        ValidLocation(LocOfRespWrite(respWrites[id]))
+  }
+
+  predicate respReadsHaveValidLocations(respReads: map<D.ReqId, D.RespRead>)
+  {
+    forall id | id in respReads ::
+        && |respReads[id].bytes| < 0x1_0000_0000_0000_0000
+        && ValidLocation(LocOfRespRead(respReads[id]))
+  }
+
+  predicate respReadHasCorrectData(contents: seq<byte>, respRead: D.RespRead)
+  {
+    && |respRead.bytes| < 0x1_0000_0000_0000_0000
+    && locInBounds(LocOfRespRead(respRead), contents)
+    && atLoc(LocOfRespRead(respRead), contents)
+        == respRead.bytes
+  }
+
+  predicate respReadsHaveCorrectData(contents: seq<byte>, respReads: map<D.ReqId, D.RespRead>)
+  {
+    forall id | id in respReads ::
+        respReadHasCorrectData(contents, respReads[id])
+  }
+
+  predicate writesOverlap(r1: D.ReqWrite, r2: D.ReqWrite)
+  requires |r1.bytes| < 0x1_0000_0000_0000_0000
+  requires |r2.bytes| < 0x1_0000_0000_0000_0000
+  {
+    overlap(LocOfReqWrite(r1), LocOfReqWrite(r2))
+  }
+
+  predicate allWritesDontOverlap(reqWrites: map<D.ReqId, D.ReqWrite>)
+  requires reqWritesHaveValidLocations(reqWrites)
+  {
+    forall id1, id2 ::
+      id1 in reqWrites && id2 in reqWrites && id1 != id2
+      ==> !writesOverlap(reqWrites[id1], reqWrites[id2])
+  }
+
+  predicate writeReqReadOverlap(r1: D.ReqWrite, r2: D.ReqRead)
+  requires |r1.bytes| < 0x1_0000_0000_0000_0000
+  {
+    overlap(LocOfReqWrite(r1), LocOfReqRead(r2))
+  }
+
+  predicate allWritesReqReadsDontOverlap(reqWrites: map<D.ReqId, D.ReqWrite>, reqReads: map<D.ReqId, D.ReqRead>)
+  requires reqWritesHaveValidLocations(reqWrites)
+  {
+    forall id1, id2 ::
+      id1 in reqWrites && id2 in reqReads
+      ==> !writeReqReadOverlap(reqWrites[id1], reqReads[id2])
+  }
+
+  predicate writeRespReadOverlap(r1: D.ReqWrite, r2: D.RespRead)
+  requires |r1.bytes| < 0x1_0000_0000_0000_0000
+  requires |r2.bytes| < 0x1_0000_0000_0000_0000
+  {
+    overlap(LocOfReqWrite(r1), LocOfRespRead(r2))
+  }
+
+  predicate allWritesRespReadsDontOverlap(reqWrites: map<D.ReqId, D.ReqWrite>, respReads: map<D.ReqId, D.RespRead>)
+  requires reqWritesHaveValidLocations(reqWrites)
+  requires respReadsHaveValidLocations(respReads)
+  {
+    forall id1, id2 ::
+      id1 in reqWrites && id2 in respReads
+      ==> !writeRespReadOverlap(reqWrites[id1], respReads[id2])
+  }
+
+  ///// respWrites are correct
+
+  predicate respWritesHaveValidNodes(contents: seq<byte>, respWrites: map<D.ReqId, D.RespWrite>)
+  {
+    forall id | id in respWrites ::
+        ValidNodeLocation(LocOfRespWrite(respWrites[id])) ==>
+          && locInBounds(LocOfRespWrite(respWrites[id]), contents)
+          && ValidNodeBytes(atLoc(LocOfRespWrite(respWrites[id]), contents))
+  }
+
+  predicate respWritesHaveValidIndirectionTables(contents: seq<byte>, respWrites: map<D.ReqId, D.RespWrite>)
+  {
+    forall id | id in respWrites ::
+        ValidIndirectionTableLocation(LocOfRespWrite(respWrites[id])) ==>
+          && locInBounds(LocOfRespWrite(respWrites[id]), contents)
+          && ValidIndirectionTableBytes(atLoc(LocOfRespWrite(respWrites[id]), contents))
+  }
+
+  predicate respWritesHaveValidJournals(contents: seq<byte>, respWrites: map<D.ReqId, D.RespWrite>)
+  {
+    forall id | id in respWrites ::
+        ValidJournalLocation(LocOfRespWrite(respWrites[id])) ==>
+          && locInBounds(LocOfRespWrite(respWrites[id]), contents)
+          && ValidJournalBytes(atLoc(LocOfRespWrite(respWrites[id]), contents))
+  }
+
+  predicate respWritesHaveValidSuperblocks(contents: seq<byte>, respWrites: map<D.ReqId, D.RespWrite>)
+  {
+    forall id | id in respWrites ::
+        ValidSuperblockLocation(LocOfRespWrite(respWrites[id])) ==>
+          && locInBounds(LocOfRespWrite(respWrites[id]), contents)
+          && ValidSuperblockBytes(atLoc(LocOfRespWrite(respWrites[id]), contents))
+  }
+
+  predicate respWritesHaveValidData(contents: seq<byte>, respWrites: map<D.ReqId, D.RespWrite>)
+  {
+    && respWritesHaveValidNodes(contents, respWrites)
+    && respWritesHaveValidIndirectionTables(contents, respWrites)
+    && respWritesHaveValidJournals(contents, respWrites)
+    && respWritesHaveValidSuperblocks(contents, respWrites)
+  }
+
+  ///// Define Inv
+
+  predicate Inv(k: Constants, s: Variables)
+  {
+    && reqWritesHaveValidLocations(s.disk.reqWrites)
+    && reqReadsHaveValidLocations(s.disk.reqReads)
+    && respWritesHaveValidLocations(s.disk.respWrites)
+    && respReadsHaveValidLocations(s.disk.respReads)
+    && respReadsHaveCorrectData(s.disk.contents, s.disk.respReads)
+    && reqWritesHaveValidData(s.disk.reqWrites)
+    && respWritesHaveValidData(s.disk.contents, s.disk.respWrites)
+    && allWritesDontOverlap(s.disk.reqWrites)
+    && allWritesReqReadsDontOverlap(s.disk.reqWrites, s.disk.reqReads)
+    && allWritesRespReadsDontOverlap(s.disk.reqWrites, s.disk.respReads)
+    && BetreeJournalSystem.Inv(Ik(k), I(k, s))
+  }
+  
+  lemma InitImpliesInv(k: Constants, s: Variables)
+    // Inherited from abstract module:
+    //requires Init(k, s)
+    //ensures Inv(k, s)
+  {
+    BetreeJournalSystem.InitImpliesInv(Ik(k), I(k, s));
+  }
+
+  lemma ReqReadStepPreservesInv(k: Constants, s: Variables, s': Variables, uiop: UIOp, dop: DiskOp)
+    requires Inv(k, s)
+    requires Machine(k, s, s', uiop, dop)
+    requires dop.ReqReadOp?
+    ensures Inv(k, s')
+  {
+  }
+
+  lemma ReqWriteStepPreservesInv(k: Constants, s: Variables, s': Variables, uiop: UIOp, dop: DiskOp)
+    requires Inv(k, s)
+    requires Machine(k, s, s', uiop, dop)
+    requires dop.ReqWriteOp?
+    ensures Inv(k, s')
+  {
+  }
+
+  lemma ReqWrite2StepPreservesInv(k: Constants, s: Variables, s': Variables, uiop: UIOp, dop: DiskOp)
+    requires Inv(k, s)
+    requires Machine(k, s, s', uiop, dop)
+    requires dop.ReqWrite2Op?
+    ensures Inv(k, s')
+  {
+  }
+
+  lemma RespReadStepPreservesInv(k: Constants, s: Variables, s': Variables, uiop: UIOp, dop: DiskOp)
+    requires Inv(k, s)
+    requires Machine(k, s, s', uiop, dop)
+    requires dop.RespReadOp?
+    ensures Inv(k, s')
+  {
+  }
+
+  lemma RespWriteStepPreservesInv(k: Constants, s: Variables, s': Variables, uiop: UIOp, dop: DiskOp)
+    requires Inv(k, s)
+    requires Machine(k, s, s', uiop, dop)
+    requires dop.RespWriteOp?
+    ensures Inv(k, s')
+  {
+  }
+
+  lemma NoDiskOpStepPreservesInv(k: Constants, s: Variables, s': Variables, uiop: UIOp, dop: DiskOp)
+    requires Inv(k, s)
+    requires Machine(k, s, s', uiop, dop)
+    requires dop.NoDiskOp?
+    ensures Inv(k, s')
+  {
+  }
+
+  lemma MachineStepPreservesInv(k: Constants, s: Variables, s': Variables, uiop: UIOp, dop: DiskOp)
+    requires Inv(k, s)
+    requires Machine(k, s, s', uiop, dop)
+    ensures Inv(k, s')
+  {
+    match dop {
+      case ReqReadOp(_, _) => ReqReadStepPreservesInv(k, s, s', uiop, dop);
+      case ReqWriteOp(_, _) => ReqWriteStepPreservesInv(k, s, s', uiop, dop);
+      case ReqWrite2Op(_, _, _, _) => ReqWrite2StepPreservesInv(k, s, s', uiop, dop);
+      case RespReadOp(_, _) => RespReadStepPreservesInv(k, s, s', uiop, dop);
+      case RespWriteOp(_, _) => RespWriteStepPreservesInv(k, s, s', uiop, dop);
+      case NoDiskOp => NoDiskOpStepPreservesInv(k, s, s', uiop, dop);
+    }
+  }
+
+  lemma DiskInternalStepPreservesInv(k: Constants, s: Variables, s': Variables, uiop: UIOp, step: D.InternalStep)
+    requires Inv(k, s)
+    requires DiskInternal(k, s, s', uiop, step)
+    ensures Inv(k, s')
+  {
+  }
+
+  lemma CrashStepPreservesInv(k: Constants, s: Variables, s': Variables, uiop: UIOp)
+    requires Inv(k, s)
+    requires Crash(k, s, s', uiop)
+    ensures Inv(k, s')
+  {
+  }
+
+  lemma NextStepPreservesInv(k: Constants, s: Variables, s': Variables, uiop: UIOp, step: Step)
+    requires Inv(k, s)
+    requires NextStep(k, s, s', uiop, step)
+    ensures Inv(k, s')
+  {
+    match step {
+      case MachineStep(dop) => MachineStepPreservesInv(k, s, s', uiop, dop);
+      case DiskInternalStep(step) => DiskInternalStepPreservesInv(k, s, s', uiop, step);
+      case CrashStep => CrashStepPreservesInv(k, s, s', uiop);
+    }
+  }
+
+  lemma NextPreservesInv(k: Constants, s: Variables, s': Variables, uiop: UIOp)
+    // Inherited from abstract module:
+    //requires Inv(k, s)
+    //requires Next(k, s, s', uiop)
+    //ensures Inv(k, s')
+  {
+    var step :| NextStep(k, s, s', uiop, step);
+    NextStepPreservesInv(k, s, s', uiop, step);
   }
 }
